coq/ZF/Set/Eval.v
@@ -1,3 +1,6 @@
+Declare Scope ZF_Set_Eval_scope.
+Open    Scope ZF_Set_Eval_scope.
+
 Require Import ZF.Class.
 Require Import ZF.Class.Eval.
 Require Import ZF.Set.
@@ -5,3 +8,6 @@ Require Import ZF.Set.FromClass.
 
 Definition eval (P:Class) (a:U) : U := fromClass (Class.Eval.eval P a)
   (EvalIsSmall P a).
+
+Notation "P :( a ):" := (eval P a)
+  (at level 0, no associativity) : ZF_Set_Eval_scope.
